src/dvspec/dafny/att_spec_proofs/dvn_next_ind_inv.dfy
@@ -6,6 +6,7 @@ include "../specification/dvn.dfy"
 include "../att_spec_proofs/inv.dfy"
 include "../att_spec_proofs/assump.dfy"
 include "../att_spec_proofs/dvc_ind_inv.dfy"
+include "../att_spec_proofs/fnc_ind_inv.dfy"
 
 module DVN_Next_Ind_Inv
 {
@@ -18,6 +19,7 @@ module DVN_Next_Ind_Inv
     import opened Att_Inv_With_Empty_Initial_Attestation_Slashing_DB
     import opened Att_Assumptions
     import opened DVN_Ind_Inv
+    import opened Fnc_Ind_Inv
 
     lemma {:axiom} dvn_next_event_inv5_axiom(dvn: DVState, e: DV.Event, dvn': DVState)       
     requires DV.NextEvent(dvn, e, dvn')        
@@ -82,30 +84,117 @@ module DVN_Next_Ind_Inv
         }        
     }
 
-    lemma dvn_next_inv1(dvn: DVState, dvn': DVState)       
+    lemma lemma_dvn_next_inv1(dvn: DVState, dvn': DVState)       
     requires exists e: DV.Event :: DV.NextEvent(dvn, e, dvn')
     requires inv1(dvn)
     ensures inv1(dvn')
     { }
 
-    lemma dvn_next_inv2(dvn: DVState, dvn': DVState)       
+    lemma lemma_dvn_next_inv2(dvn: DVState, dvn': DVState)       
     requires exists e: DV.Event :: DV.NextEvent(dvn, e, dvn')
     requires inv2(dvn)
     ensures inv2(dvn')
     { }
 
-    lemma dvn_next_inv3(dvn: DVState, dvn': DVState)       
-    requires exists e: DV.Event :: DV.NextEvent(dvn, e, dvn')
+    lemma {:axiom} assump_lemma_dvn_next_inv3(
+        s': DVState
+    )
+    ensures inv3(s')
+
+    lemma lemma_dvn_next_inv3(
+        dvn: DVState,
+        event: DV.Event,
+        dvn': DVState
+    )
+    requires inv1(dvn)
+    requires unchanged_fixed_paras(dvn, dvn')
+    requires NextEvent(dvn, event, dvn')
     requires inv3(dvn)
     ensures inv3(dvn')
-    { }
+    {
+        match event 
+        {
+            case HonestNodeTakingStep(node, nodeEvent, nodeOutputs) =>
+                var dvc := dvn.honest_nodes_states[node];
+                var dvc' := dvn'.honest_nodes_states[node];
+                match nodeEvent
+                {
+                    case ServeAttstationDuty(att_duty) =>            
+                        forall hn | hn in dvn.honest_nodes_states.Keys                        
+                        ensures forall duty: AttestationDuty 
+                                    | 
+                                    duty in dvn'.honest_nodes_states[hn].all_rcvd_duties
+                                    ::
+                                    exists k: nat :: 
+                                        && dvn'.sequence_attestation_duties_to_be_served[k].node == hn
+                                        && dvn'.sequence_attestation_duties_to_be_served[k].attestation_duty == duty
+                                        
+                        {
+                            if hn != node 
+                            {
+                                assert dvn.sequence_attestation_duties_to_be_served == dvn'.sequence_attestation_duties_to_be_served;                          
+                                assert dvn'.honest_nodes_states[hn].all_rcvd_duties == dvn.honest_nodes_states[hn].all_rcvd_duties;                                                                  
+                                assert forall duty: AttestationDuty 
+                                                | 
+                                                duty in dvn'.honest_nodes_states[hn].all_rcvd_duties
+                                                ::
+                                                exists k: nat :: 
+                                                    && dvn'.sequence_attestation_duties_to_be_served[k].node == hn
+                                                    && dvn'.sequence_attestation_duties_to_be_served[k].attestation_duty == duty                              
+                                ;                                                                                             
+                            }
+                            else 
+                            {   
+                                var curr_index := dvn.index_next_attestation_duty_to_be_served;
+                                var new_duty := dvn.sequence_attestation_duties_to_be_served[curr_index].attestation_duty;
+                                assert node == dvn.sequence_attestation_duties_to_be_served[curr_index].node;                        
+                                lemma_f_serve_attestation_duty_inv3(dvc, new_duty, dvc');    
+                                assert dvc'.all_rcvd_duties == dvc.all_rcvd_duties + {new_duty};                                                            
+                                                                                          
+                                forall duty: AttestationDuty | duty in dvn'.honest_nodes_states[hn].all_rcvd_duties
+                                ensures exists k: nat :: 
+                                                && dvn'.sequence_attestation_duties_to_be_served[k].node == hn
+                                                && dvn'.sequence_attestation_duties_to_be_served[k].attestation_duty == duty                              
+                                {
+                                    if duty == new_duty
+                                    {                                                                              
+                                        assert && dvn'.sequence_attestation_duties_to_be_served[curr_index].node == hn
+                                               && dvn'.sequence_attestation_duties_to_be_served[curr_index].attestation_duty == duty;
+                                        
+                                        assert exists k: nat :: 
+                                                && dvn'.sequence_attestation_duties_to_be_served[k].node == hn
+                                                && dvn'.sequence_attestation_duties_to_be_served[k].attestation_duty == duty;
+                                    }
+                                    else
+                                    {                                        
+                                        assert exists k: nat :: 
+                                                && dvn'.sequence_attestation_duties_to_be_served[k].node == hn
+                                                && dvn'.sequence_attestation_duties_to_be_served[k].attestation_duty == duty;
+                                    }
+                                }                            
+                            }
+                        }
+                        
+                    case AttConsensusDecided(id, decided_attestation_data) => 
+                        lemma_f_att_consensus_decided_inv3(dvc, id, decided_attestation_data, dvc');
+                        
+                    case ReceviedAttesttionShare(attestation_share) => 
+                        lemma_f_listen_for_attestation_shares_inv3(dvc, attestation_share, dvc');
+   
+                    case ImportedNewBlock(block) => 
+                        var dvc := add_block_to_bn(dvc, nodeEvent.block);
+                        lemma_f_listen_for_new_imported_blocks_inv3(dvc, block, dvc');
+                        
+                    case ResendAttestationShares => 
+                        
+                    case NoEvent => 
+                        
+                }
 
-    lemma dvn_next_inv4(dvn: DVState, dvn': DVState)       
-    requires exists e: DV.Event :: DV.NextEvent(dvn, e, dvn')
-    requires inv4(dvn)
-    ensures inv4(dvn')
-    { }
-
+            case AdeversaryTakingStep(node, new_attestation_share_sent, messagesReceivedByTheNode) =>
+                
+        }        
+    }   
     
     
  
