src/dvspec/dafny/specification/dvn.dfy
@@ -97,6 +97,7 @@ module DV
         att_shares: set<AttestationShare>,
         data: AttestationData
     )       
+    requires construct_signed_attestation_signature(att_shares).isPresent()
     {
         && var fork_version := bn_get_fork_version(compute_start_slot_at_epoch(data.target.epoch));
         && var signing_root := compute_attestation_signing_root(data, fork_version);
@@ -295,6 +296,7 @@ module DV
         nodeOutputs: DVCNode_Spec.Outputs,
         s': DVState        
     ) 
+    requires unchanged_fixed_paras(s, s')
     {
         && node in s.honest_nodes_states.Keys        
         && var s_w_honest_node_states_updated :=
@@ -315,6 +317,7 @@ module DV
         nodeOutputs: DVCNode_Spec.Outputs,
         s': DVState
     )
+    requires unchanged_fixed_paras(s, s')
     {
         && node in s.honest_nodes_states.Keys 
         && var new_node_state := s'.honest_nodes_states[node];
